\documentclass{article}
\usepackage{amsmath}
\usepackage{graphicx}
\usepackage{amssymb}
\begin{document}
\begin{enumerate}
    \item
        First, we compute the derivatives of the exact solution: \\
        \begin{equation*}
            \begin{split}
                u(t)  & = \eta e^{-\lambda t} \\
                u'(t) & = -\lambda \eta e^{-\lambda t} \\
                u''(t) & = \lambda^2 \eta e^{-\lambda t} \\
            \end{split}
        \end{equation*}
        Then, the Taylor series method sequence is: \\
        \begin{equation*}
            \begin{split}
                U^0     & = u(0) = \eta \\
                U^{n+1} & = U^n + ku'(kn) + \dfrac{1}{2}k^2u''(kn) \\
                        & = U^n - k\lambda \eta e^{-\lambda kn} + \dfrac{1}{2}k^2\lambda^2\eta e^{\lambda kn} \\
                        & = U^n + k\lambda \eta e^{-\lambda kn} \left( \dfrac{k\lambda}{2} - 1 \right) \\
            \end{split}
        \end{equation*}
        For $k\lambda > 0$, $-kn\lambda$ will approach $-\infty$ for large $n$ and therefore $e^{-kn\lambda}$ approaches $0$. \\
        As a result the change from $U^n$ to $U^{n+1}$ will approach $0$ and the approximation must decay. \\
    \item
        \begin{enumerate}
            \item
                \begin{equation*}
                    \begin{split}
                        u'   & = u - t^2 + 1 \\
                        u(0) & = 0 \\
                        u(t) & = c_1e^t + t^2 + 2t + 1 \\
                             & = -e^t + t^2 + 2t + 1 \\
                    \end{split}
                \end{equation*}
            \item
                The derivatives for the exact solution are as follows: \\
                \begin{equation*}
                    \begin{split}
                        u'(t)    & = -e^t + 2t + 2 \\
                        u''(t)   & = -e^t + 2 \\
                        u'''(t)  & = -e^t \\
                        u''''(t) & = -e^t \\
                    \end{split}
                \end{equation*}
                Then, the Taylor series method approximation is the following: \\
                \begin{equation*}
                    \begin{split}
                        U^0     & = u(0) = 0 \\
                        U^{n+1} & = U^n + ku'(t^n) + \dfrac{1}{2!}k^2u''(t^n) + \dfrac{1}{3!}k^3u'''(t^n) + \dfrac{1}{4!}k^4u''''(t^n) \\
                                & = U^n -ke^{t^n} + 2kt^n + 2k - \dfrac{1}{2}k^2e^{t^n} + k^2 - \dfrac{1}{6}k^3e^{t^n} - \dfrac{1}{24}k^4e^{t^n} \\
                    \end{split}
                \end{equation*}
            \item
                Results from the approximation: \\
                \begin{center}
                    \begin{tabular}{| c | c | c |}
                        \hline
                        k & error & ratio \\
                        \hline
                        0.25 & 1.9e-4 & - \\
                        0.125 & 1.24e-5 & 15.32 \\
                        0.0625 & 7.96e-7 & 15.66 \\
                        0.03125 & 5.02e-8 & 15.83 \\
                        0.015625 & 3.16e-9 & 15.91 \\
                        0.0078125 & 1.98e-10 & 15.95 \\
                        0.00390625 & 1.23e-11 & 15.97 \\
                        0.001953125 & 7.73e-13 & 16.01 \\
                        \hline
                    \end{tabular} \\
                \end{center}
                As $N$ doubles and the timestep $k$ halves, the error decreases by a consistent factor of $16$. \\
                It follows that the error can be modeled as $\dfrac{1}{16^{\log_2{n}}}$ which can be simplified to $\dfrac{1}{n^4}$. \\
                Therefore, the approximation converges at a rate of $n^4$. \\
        \end{enumerate}
    \item
        \begin{enumerate}
            \item
                See the source code at \texttt{https://github.com/codeandkey/math481-iastate-sp2020}.\\
            \item
                Results from the approximation: \\
                \begin{center}
                    \begin{tabular}{| c | c | c | c | c |}
                        \hline
                        k & $\theta$ error & $\theta$ error ratio & $\theta'$ error & $\theta'$ error ratio \\
                        \hline
                        0.1 & 0.055 & - & 0.926 & - \\
                        0.05 & 0.013 & 4.19 & 0.220 & 4.191 \\
                        0.025 & 0.003 & 3.50 & 0.05 & 4.06 \\
                        0.0125 & 0.001 & 3.642 & 0.013 & 4.033 \\
                        0.00625 & 0.0002 & 3.79 & 0.0033 & 4.014 \\
                        0.003125 & 7.09e-5 & 3.869 & 0.0008 & 3.984 \\
                        0.0015625 & 1.844e-5 & 3.845 & 0.0002 & 3.901 \\
                        \hline
                    \end{tabular} \\
                \end{center}
        \end{enumerate}
\end{enumerate}
\end{document}
